# Lecture 11 Problems - Solutions

1. $(x^{MkII}, y^{MkII}) = (-x^{MkIII}, -y^{MkIII})$

2.
$$
   \begin{align*}
   x' &= \frac{-x_w}{z_w}\\
   y' &= \frac{-y_w}{z_w}\\
   z' &= -1
   \end{align*}
$$

3.
$$
   \begin{bmatrix} 1 & 0 & 0 \\
   0 & 1 & 0\\
   0 & 0 & 1 \end{bmatrix}
$$

4.
$$
\begin{align*}
   x' &= \frac{-fx_w}{z_w}\\
   y' &= \frac{-fy_w}{z_w}\\
   z' &= -f
   \end{align*}
$$

5.
$$
   \begin{bmatrix} x_c \\ y_c \\ 1 \end{bmatrix} \equiv
   \begin{bmatrix}\frac{-f x_w}{z_w} \\  \frac{-f y_w}{z_w} \\ 1\end{bmatrix} \sim
   \begin{bmatrix}-fx_w \\ -fy_w \\ z_w \\\end{bmatrix}_{3\times 1} =
   \begin{bmatrix} -f & 0 & 0 \\ 0 & -f & 0 \\ 0 & 0 & 1 \\\end{bmatrix}_{3\times3}
   \begin{bmatrix} x_w \\ y_w \\ z_w \end{bmatrix}
$$

6. 6a: $x_w$; 6b: $b - x_w$

7. Similar triangles - use height over height equals width over width for the top 2 and bottom 2 triangles. Solve both for $x_w$, then equate and solve for $z_w$.

   Camera 1:
   $$
   \frac{z_w}{f} = \frac{x_w}{x_L}\\
   \frac{z_w x_L}{f} = x_w
   $$
   Camera 2:
   $$
   \frac{b-x_w}{x_R} = \frac{z_w}{f}\\
   x_w = b - \frac{z_w x_r}{f}
   $$
   Equate $x_w = x_w$:
   $$
   \frac{z_w x_L}{f} = b - \frac{z_w x_R}{f}
   $$
   (... some algebra...)
   $$
   z_w = \frac{fb}{x_L-x_R}
   $$
